DL/PoK.ec
@@ -1,20 +1,22 @@
 pragma Goals:printall.
 require import AllCore DBool Bool List Distr Aux Finite.
-require import Basics.
 
+require import CyclicGroup.
+
+require import Basics.
 require import SpecialSoundness.
 clone import PoK.
 
-require import CyclicGroup.
-import FDistr.
-clone import ComputationalPoK with op special_soundness_extract <- special_soundness_extract.
 
+import FDistr.
+clone import ComputationalPoK with op special_soundness_extract <- special_soundness_extract. (* should not be needed after statistical_PoK is "moved" to SpecialSoundness  *)
 
 section.
-declare module P : MaliciousProver {HonestVerifier}.
+declare module P : MaliciousProver{HonestVerifier}.
 
 axiom P_response_ll : islossless P.response.
 
+  (* Would be available as SpecialSoundness.statistical_PoK *)
 lemma dl_computational_PoK &m  s aux: 
   Pr[Extractor(P).extract(s, aux) @ &m : IsDL s res ] >=
    (Pr[Soundness(P, HonestVerifier).run(s, aux) @ &m : res]^2
