program_logic/GenericKE.ec
@@ -1,0 +1,364 @@
+pragma Goals:printall.
+require import AllCore Distr List Binomial.
+require import Ring StdRing StdOrder StdBigop Discrete RealSeq RealSeries RealLub.
+(*---*) import IterOp Bigint Bigreal Bigreal.BRA.
+(*---*) import IntOrder RealOrder RField.
+require (*--*) FinType.
+
+require import AllpairsProp.
+
+
+type ct, pt, rt, irt, auxt.
+
+op d : ct distr.
+axiom duni : is_uniform d.
+
+op allcs : ct list.
+axiom allcs_uniq : uniq allcs.
+
+axiom ss c : mu1 d c = 1%r/(size allcs)%r.
+
+require BigPr.
+clone import BigPr as BP with type ct  <- ct,
+                              type pt  <- pt * auxt,
+                              type rt  <- (rt * irt) * (rt * irt),
+                              op    d  <- d,
+                              op allcs <- allcs.
+
+module type Adv = {
+  proc init(p : pt, aux : auxt) : irt
+  proc run(i : irt, c : ct)  : rt
+}.
+
+
+
+module InitRun2(A : Adv) = {
+  proc run(a : pt, aux : auxt) = {
+    var i, c1, c2, r1, r2;
+    i <- A.init(a,aux);
+    
+    c1 <$ d;
+    r1 <- A.run(i,c1);
+
+    c2 <$ d;
+    r2 <- A.run(i,c2);
+
+    return ((c1,(r1,i)),(c2,(r2,i)));
+  }
+}.
+
+
+module InitRun1(A : Adv) = {
+  proc run(a : pt, aux : auxt) = {
+    var i, c1, r1;
+    i <- A.init(a,aux);
+    
+    c1 <$ d;
+    r1 <- A.run(i,c1);
+
+    return (c1,(r1,i));
+  }
+}.
+
+
+section.
+declare module A : Adv.
+
+axiom A_ll : islossless A.run.
+
+local module C2 : Comp = {
+  proc rest(p : pt * auxt, c1c2 : ct * ct) : (rt * irt) * (rt * irt) = {
+    var r1, r2,i;
+    i  <@ A.init(p);
+    r1 <@ A.run(i,c1c2.`1);
+    r2 <@ A.run(i,c1c2.`2);
+    return ((r1,i),(r2,i));
+  }
+}.
+
+
+local module C1 = {
+  proc rest(p : pt * auxt, c1 : ct) : rt * irt = {
+    var r1,i;
+    i  <@ A.init(p);
+    r1 <@ A.run(i,c1);
+    return (r1,i);
+  }
+}.
+
+local module X1 = {
+  proc run(p : pt * auxt) = {
+    var c,r;
+    c <$ d;
+    r <- C1.rest(p,c);
+    return (c,r);
+  }
+}.
+
+
+(* averging  *)
+local lemma x0 &m M p : 
+  big predT (fun (c : ct) => mu1 d c * Pr[C1.rest(p, c) @ &m : M p (c, res)]) allcs =
+     Pr[X1.run(p) @ &m : M p (res.`1, res.`2)].
+admitted.
+
+
+(* c1c2 <$ d * d ~ c1 <$ d ; c2 <$ d  *)
+local lemma x1 &m M p: 
+   Pr[X(C2).run(p) @ &m : M p res] = Pr[Xseq(C2).run(p) @ &m : M p res].
+admitted.
+
+
+   
+(* sum binding  *)
+local lemma x2 &m M p:
+  Pr[X1.run(p) @ &m : M p (res.`1, res.`2)] ^ 2 <=
+  Pr[Xseq(C2).run(p) @ &m : M p (res.`1.`1, res.`2.`1) /\ M p (res.`1.`2, res.`2.`2)].
+admitted.
+   
+
+local lemma avr_lemma_6_app &m M p : 
+  Pr[ Xseq(C2).run(p) @ &m  : res.`1.`1 <> res.`1.`2 /\ M p res ] 
+     = Pr[ Xseq(C2).run(p) @ &m  : M p res ] 
+     - big (fun r => fst r = snd r)  (fun (c1c2 : ct * ct) => 
+                  ((mu1 d c1c2.`1) * (mu1 d c1c2.`2)) * 
+                   Pr[ C2.rest(p,c1c2) @ &m :  M p (c1c2,res) ]) 
+                   (cartprod2 allcs).
+rewrite -  (x1 &m (fun p (r :  (ct * ct) * ((rt * irt) * (rt * irt))) => r.`1.`1 <> r.`1.`2 /\ M p r)).
+rewrite (avr_lemma_6 C2 &m (M p) p).
+rewrite - x1. auto.
+qed.
+
+
+local lemma avr_lemma_7_app &m M p c: 
+ Pr[ C2.rest(p,(c,c)) @ &m :  M p (c, res.`1) /\ M p (c, res.`2) ]
+  <= Pr[ C1.rest(p,c) @ &m :  M p (c, res) ].
+byequiv.
+proc.
+seq 2 2 : (={glob A,i,r1}).
+call (_:true). call (_:true). skip. progress.
+call {1} (_: true ==> true). apply A_ll. skip. progress. auto.
+auto.
+qed.
+
+
+local lemma avr_lemma_8_app &m M p : 
+  Pr[ Xseq(C2).run(p) @ &m  : res.`1.`1 <> res.`1.`2 /\ M p (res.`1.`1, res.`2.`1) /\ M p (res.`1.`2, res.`2.`2) ] 
+
+     >= Pr[ Xseq(C2).run(p) @ &m  : M p (res.`1.`1, res.`2.`1) /\ M p (res.`1.`2, res.`2.`2)  ] 
+     - big (fun r => fst r = snd r)  (fun (c1c2 : ct * ct) => 
+                  ((mu1 d c1c2.`1) * (mu1 d c1c2.`2)) * 
+                   Pr[ C1.rest(p,c1c2.`1) @ &m :  M p (c1c2.`1, res) ]) 
+                   (cartprod2 allcs).
+rewrite (avr_lemma_6_app &m (fun p (r :  (ct * ct) * ((rt * irt) * (rt * irt))) =>   M p (r.`1.`1, r.`2.`1) /\ M p (r.`1.`2, r.`2.`2))).
+simplify.
+have f2 :  big (fun (r : ct * ct) => r.`1 = r.`2)
+  (fun (c1c2 : ct * ct) =>
+     mu1 d c1c2.`1 * mu1 d c1c2.`2 *
+     Pr[C2.rest(p, c1c2) @ &m : M p (c1c2.`1, res.`1) /\ M p (c1c2.`2, res.`2)])
+  (cartprod2 allcs) <= 
+  big (fun (r : ct * ct) => r.`1 = r.`2)
+  (fun (c1c2 : ct * ct) =>
+     mu1 d c1c2.`1 * mu1 d c1c2.`2 *
+     Pr[C1.rest(p, c1c2.`1) @ &m : M p (c1c2.`1, res)]) (cartprod2 allcs).
+apply ler_sum. progress. 
+   have : Pr[C2.rest(p, a) @ &m : M p (a.`1, res.`1) /\ M p (a.`2, res.`2)] <=
+            Pr[C1.rest(p, a.`1) @ &m : M p (a.`1, res)].
+    rewrite H.
+      have ->: a = (a.`1,a.`1).  smt. simplify.
+      apply (avr_lemma_7_app &m M p ). 
+     smt.
+have f3  : forall (a b c : real), b <= c => a - b >= a - c.
+smt.
+apply f3.
+apply f2.
+qed.
+
+
+local lemma avr_lemma_9_app &m M p : 
+     big (fun r => fst r = snd r)  (fun (c1c2 : ct * ct) => 
+                  ((mu1 d c1c2.`1) * (mu1 d c1c2.`2)) * 
+                    Pr[ C1.rest(p,c1c2.`1) @ &m :  M p (c1c2.`1, res) ]) 
+                    (cartprod2 allcs)
+     = (1%r/(size allcs)%r) * Pr[ X1.run(p) @ &m :  M p (res.`1, res.`2) ].
+have ->: big (fun r => fst r = snd r)  (fun (c1c2 : ct * ct) => 
+                  ((mu1 d c1c2.`1) * (mu1 d c1c2.`2)) * 
+                   Pr[ C1.rest(p,c1c2.`1) @ &m :  M p (c1c2.`1, res) ]) 
+                   (cartprod2 allcs)
+      = big (fun r => fst r = snd r)  (fun (c1c2 : ct * ct) => 
+                  (1%r/(size allcs)%r) * ((mu1 d c1c2.`1) * 
+                   Pr[ C1.rest(p,c1c2.`1) @ &m :  M p (c1c2.`1, res) ])) 
+                   (cartprod2 allcs).
+apply eq_big. auto. 
+progress.
+rewrite ss. rewrite ss. simplify. auto. simplify. 
+have ->: big (fun (r : ct * ct) => r.`1 = r.`2)
+  (fun (c1c2 : ct * ct) =>
+     (1%r/(size allcs)%r) * (mu1 d c1c2.`1 * Pr[C1.rest(p, c1c2.`1) @ &m : M p (c1c2.`1, res)]))
+  (cartprod2 allcs)
+ = (1%r/(size allcs)%r) * big (fun (r : ct * ct) => r.`1 = r.`2)
+  (fun (c1c2 : ct * ct) =>
+      (mu1 d c1c2.`1 * Pr[C1.rest(p, c1c2.`1) @ &m : M p (c1c2.`1, res)]))
+  (cartprod2 allcs).
+rewrite mulr_sumr. auto.
+auto.
+have ->: big (fun (r : ct * ct) => r.`1 = r.`2)
+  (fun (c1c2 : ct * ct) =>
+     mu1 d c1c2.`1 * Pr[C1.rest(p, c1c2.`1) @ &m : M p (c1c2.`1, res)])
+  (cartprod2 allcs)
+   = big predT
+      (fun (c : ct) =>
+         mu1 d c * Pr[C1.rest(p, c) @ &m : M p (c, res)])
+          allcs.
+have ->: big predT (fun (c : ct) => mu1 d c * Pr[C1.rest(p, c) @ &m : M p (c, res)]) allcs = big predT (fun (c : ct) => mu1 d c * Pr[C1.rest(p, c) @ &m : M p (c, res)]) 
+    (map fst (filter (fun x => fst x = snd x) (cartprod2 allcs))). rewrite cart2_diag_unzip1. smt. auto.
+rewrite big_mapT. 
+rewrite - big_filter. rewrite  /(\o). auto.
+ rewrite x0. auto.
+qed.
+
+
+local lemma avr_lemma_10_app &m M p : 
+  Pr[ Xseq(C2).run(p) @ &m  : res.`1.`1 <> res.`1.`2 /\ M p (res.`1.`1, res.`2.`1) /\ M p (res.`1.`2, res.`2.`2) ] >= 
+  Pr[ Xseq(C2).run(p) @ &m  : M p (res.`1.`1, res.`2.`1) /\ M p (res.`1.`2, res.`2.`2)  ] 
+   - (1%r/(size allcs)%r) * Pr[ X1.run(p) @ &m :  M p (res.`1, res.`2) ].
+rewrite - avr_lemma_9_app.
+apply avr_lemma_8_app.
+qed.
+
+
+local lemma avr_lemma_11_app &m M p : 
+   Pr[ Xseq(C2).run(p) @ &m  : res.`1.`1 <> res.`1.`2 
+            /\ M p (res.`1.`1, res.`2.`1) /\ M p (res.`1.`2, res.`2.`2) ] 
+       >= Pr[ X1.run(p) @ &m :  M p (res.`1, res.`2) ] ^2
+          - (1%r/(size allcs)%r) * Pr[ X1.run(p) @ &m :  M p (res.`1, res.`2) ].
+apply (ler_trans (Pr[ Xseq(C2).run(p) @ &m  : M p (res.`1.`1, res.`2.`1) 
+                                             /\ M p (res.`1.`2, res.`2.`2)  ] 
+   - (1%r/(size allcs)%r) * Pr[ X1.run(p) @ &m :  M p (res.`1, res.`2) ])). 
+have ff : Pr[X1.run(p) @ &m : M p (res.`1, res.`2)] ^ 2
+     <= Pr[Xseq(C2).run(p) @ &m : M p (res.`1.`1, res.`2.`1) 
+                                     /\ M p (res.`1.`2, res.`2.`2)].
+apply x2.
+smt. 
+apply (avr_lemma_10_app &m M p).
+qed.
+
+
+lemma final_eq &m M p : 
+   Pr[ InitRun2(A).run(p) @ &m 
+          : res.`1.`1 <> res.`2.`1 /\ M p res.`1 /\ M p res.`2 ] 
+  >= Pr[ InitRun1(A).run(p) @ &m  :  M p res ]^2
+          - (1%r/(size allcs)%r) * Pr[ InitRun1(A).run(p) @ &m  :  M p res ].
+proof.
+ have <-: Pr[ Xseq(C2).run(p) @ &m  : res.`1.`1 <> res.`1.`2 
+            /\ M p (res.`1.`1, res.`2.`1) /\ M p (res.`1.`2, res.`2.`2) ] 
+    = Pr[ InitRun2(A).run(p) @ &m 
+          : res.`1.`1 <> res.`2.`1 /\ M p res.`1 /\ M p res.`2 ].
+byequiv. proc.  simplify.
+swap {2} 2 -1.
+swap {2} 4 -2.
+inline*. wp. 
+call (_:true).
+call (_:true).
+call (_:true). wp.  simplify.
+rnd. rnd.
+skip. progress. auto.  auto.
+ have <-: Pr[ X1.run(p) @ &m :  M p (res.`1, res.`2) ] 
+    = Pr[ InitRun1(A).run(p) @ &m : M p res ].
+byequiv. proc. inline*. swap {2} 2 -1. wp. 
+simplify.   call (_:true).  call (_:true). wp. rnd. 
+skip. progress. auto.  auto. 
+apply avr_lemma_11_app.
+qed.
+
+
+lemma final_eq_step1 &m AccRun SuccExtr p negl : 
+   Pr[ InitRun2(A).run(p) @ &m 
+          : res.`1.`1 <> res.`2.`1 /\ AccRun p res.`1 /\ AccRun p res.`2
+   /\ !SuccExtr p res.`1 res.`2 ] <= negl
+  => 
+   Pr[ InitRun2(A).run(p) @ &m : res.`1.`1 <> res.`2.`1 
+            /\ AccRun p res.`1 /\ AccRun p res.`2 /\ SuccExtr p res.`1 res.`2 ] 
+    >= (Pr[ InitRun1(A).run(p) @ &m  :  AccRun p res ]^2
+         - (1%r/(size allcs)%r) * Pr[ InitRun1(A).run(p) @ &m  :  AccRun p res ])
+        - negl.
+progress.
+have : Pr[InitRun1(A).run(p) @ &m : AccRun p res] ^ 2 -
+  Pr[InitRun1(A).run(p) @ &m : AccRun p res] / (size allcs)%r <=
+   Pr[InitRun2(A).run(p) @ &m : res.`1.`1 <> res.`2.`1 /\
+       AccRun p res.`1 /\ AccRun p res.`2 /\ SuccExtr p res.`1 res.`2] + negl.
+  apply (ler_trans    Pr[ InitRun2(A).run(p) @ &m 
+          : res.`1.`1 <> res.`2.`1 /\ AccRun p res.`1 /\ AccRun p res.`2 ] ).
+  apply final_eq.  
+rewrite Pr[mu_split SuccExtr p res.`1 res.`2]. 
+have ->: Pr[InitRun2(A).run(p) @ &m :
+   (res.`1.`1 <> res.`2.`1 /\ AccRun p res.`1 /\ AccRun p res.`2) /\
+   SuccExtr p res.`1 res.`2] = Pr[InitRun2(A).run(p) @ &m :
+   res.`1.`1 <> res.`2.`1 /\ AccRun p res.`1 /\ AccRun p res.`2 /\
+   SuccExtr p res.`1 res.`2].
+rewrite Pr[mu_eq]. smt. auto.
+have ->: Pr[InitRun2(A).run(p) @ &m :
+   (res.`1.`1 <> res.`2.`1 /\ AccRun p res.`1 /\ AccRun p res.`2) /\
+   !SuccExtr p res.`1 res.`2] = Pr[InitRun2(A).run(p) @ &m :
+   res.`1.`1 <> res.`2.`1 /\ AccRun p res.`1 /\ AccRun p res.`2 /\
+   !SuccExtr p res.`1 res.`2].
+rewrite Pr[mu_eq]. smt. auto.
+smt.
+smt.
+qed.
+
+
+require import RealExp.
+
+
+lemma qqq1  (a b : real) : a <= b  => sqrt a <= sqrt b.
+smt. qed.
+
+
+lemma qqq2  (a b : real) : a ^ 2 <= b  => a <= sqrt b.
+smt. qed.
+
+
+lemma final_eq_step2 &m AccRun SuccExtr p negl : 
+   Pr[ InitRun2(A).run(p) @ &m 
+          : res.`1.`1 <> res.`2.`1 /\ AccRun p res.`1 /\ AccRun p res.`2
+   /\ !SuccExtr p res.`1 res.`2 ] <= negl
+ => Pr[ InitRun2(A).run(p) @ &m 
+          :  SuccExtr p res.`1 res.`2 ] = 0%r   
+ => Pr[ InitRun1(A).run(p) @ &m  :  AccRun p res ]
+   <=  sqrt (negl + 1%r/(size allcs)%r).
+proof.  progress.
+have f2 :     Pr[InitRun2(A).run(p) @ &m :
+       res.`1.`1 <> res.`2.`1 /\
+  AccRun p res.`1 /\ AccRun p res.`2 /\ SuccExtr p res.`1 res.`2] = 0%r.
+  have ff2: Pr[InitRun2(A).run(p) @ &m :
+       res.`1.`1 <> res.`2.`1 /\
+  AccRun p res.`1 /\ AccRun p res.`2 /\ SuccExtr p res.`1 res.`2]
+   <= 0%r. rewrite - H0.
+   rewrite Pr[mu_sub]. smt. auto. 
+  smt.
+have f1 :    0%r 
+    >= (Pr[ InitRun1(A).run(p) @ &m  :  AccRun p res ]^2
+         - (1%r/(size allcs)%r) * Pr[ InitRun1(A).run(p) @ &m  :  AccRun p res ])
+    - negl.
+rewrite - f2.
+apply (final_eq_step1 &m). assumption.
+clear f2. clear H.
+have f3 : Pr[InitRun1(A).run(p) @ &m : AccRun p res] ^ 2 
+     <= 1%r / (size allcs)%r * Pr[InitRun1(A).run(p) @ &m : AccRun p res] + negl.
+smt.
+clear f1.
+clear H0.
+have : Pr[InitRun1(A).run(p) @ &m : AccRun p res] <=
+    sqrt (1%r / (size allcs)%r * Pr[InitRun1(A).run(p) @ &m : AccRun p res] + negl).
+apply qqq2. auto.
+clear f3. simplify.
+move => f4.
+apply (ler_trans (sqrt (Pr[InitRun1(A).run(p) @ &m : AccRun p res] / (size allcs)%r + negl))).
+auto.
+apply qqq1. smt.
+qed.
+
+
+end section.
+
